```scheme
(define (A x y) 
	(cond ((= y 0) 0) 
		((= x 0) (* 2 y)) 
		((= y 1) 2) 
		(else (A (- x 1) (A x (- y 1))))
	)
)
	  
(A 1 10) = (A 0 (A 1 9)) = (A 0 512) = 1024
(A 1 9) = (A 0 (A 1 8)) = (A 0 256) = 512
(A 1 8) = (A 0 (A 1 7)) = (A 0 128) = 256
(A 1 7) = (A 0 (A 1 6)) = (A 0 64) = 128
(A 1 6) = (A 0 (A 1 5)) = (A 0 32) = 64 
(A 1 5) = (A 0 (A 1 4)) = (A 0 16) = 32
(A 1 4) = (A 0 (A 1 3)) = (A 0 8) = 16
(A 1 3) = (A 0 (A 1 2)) = (A 0 4) =  8
(A 1 2) = (A 0 (A 1 1)) = (A 0 2) = 4
(A 1 1) = 2
```

```scheme
(A 2 4) = (A 1 (A 2 3)) = (A 1 16) = 2^16 = 2^(2^(2^2))
(A 2 3) = (A 1 (A 2 2)) = (A 1 4) = 16 = 2^4 = 2^(2^2)
(A 2 2) = (A 1 (A 2 1)) = (A 1 2) = 4 = 2^(2^1)
(A 2 1) = 2^(2^0)
```

```scheme
(A 3 3) = (A 2 (A 3 2)) = (A 2 4) = 2^16
(A 3 2) = (A 2 (A 3 1)) = (A 2 2) = 4
(A 3 1) = 2
```

```scheme
(define (f n) (A 0 n)) 
(define (g n) (A 1 n)) 
(define (h n) (A 2 n)) 
```

$$f(n)=2n$$
$$g(n)=2^{n}$$
$$h(n)=\underbrace{2^{...^{2}}}_{n}$$

